Added missing field for "this" Added missing axiom for Indexfield. Added missing free ensures on lemmas so that they don't modify the heap 302 diff count

Source/IntegrationTests/TestFiles/LitTests/LitTest/referrers/referrers-errors.dfy
@@ -25,3 +25,33 @@ method EnsuresReferrersUnchanged(t2: Test)
   var t_local := t2;
   assert referrers(t_local) == old(referrers(t_local)) + {locals`t_local}; // Error, t_local was not assigned
 }
+
+class ChainingObjectError {
+  var x: ChainingObjectError?
+  var y: ChainingObjectError?
+  ghost var nontracking: ChainingObjectError?
+  ghost var {:tracking} tracking: ChainingObjectError?
+  const tail: ChainingObjectError?
+  constructor(chained_test: ChainingObjectError?) ensures x == y == nontracking == tracking == null && tail == chained_test
+    ensures chained_test != null ==> referrers(chained_test) == old(referrers(chained_test)) + {this`tail}
+    ensures forall o: object | o != chained_test :: referrers(o) == old(referrers(o)) // Replace by referrers clauses when they arrive
+  {
+    x := null;
+    y := null;
+    tracking := null;
+    nontracking := null;
+    tail := chained_test;
+  }
+}
+
+
+method ObjectFields() {
+  var t := new ChainingObject(null);
+  var u := new ChainingObject(t);
+  // Assignment of array
+  var a := new ChainingObject[3](i => if i == 0 then t else u);
+  assert referrers(t) == {locals`t, u`tail, a`[0]};
+  assert referrers(u) == {locals`t, u`x, a`[1], a`[2]};
+
+  assert false; // There should be no contradiction.
+}
